cava/arrow-examples/Combinators.v
@@ -330,4 +330,26 @@ Section regression_tests.
     let '(carry, result) = !(rippleCarryAdder' _) b merged in
     (carry, result)
     ]>.
+  
+  Lemma interleave_is_stateless : forall n, has_no_state (interleaveVectors n EvalCava).
+  Proof.
+    intros.
+    induction n.
+    * cbv [interleaveVectors Closure_conversion closure_conversion].
+      refine (OnlyUnitsTuple _ _ OnlyUnitsUnit _ ).
+      apply (no_let_rec_and_stateless_morphisms_is_stateless _ _).
+      - cbv [Desugar desugar]; auto.
+        repeat (constructor; intros).
+      - cbv [Desugar desugar]; auto.
+        repeat (constructor; intros).
+    * cbv [interleaveVectors Closure_conversion closure_conversion].
+      refine (OnlyUnitsTuple _ _ OnlyUnitsUnit _ ).
+      apply (no_let_rec_and_stateless_morphisms_is_stateless _ _).
+      - cbv [Desugar desugar]; auto.
+        repeat (constructor; intros).
+      - cbv [Desugar desugar]; auto.
+        repeat (constructor; intros).
+        apply IHn.
+  Qed.
+
 End regression_tests.
