cava/arrow-lib/Kappa.v
@@ -7,18 +7,45 @@ Section Arrow.
     Variable (var: object -> object -> Type).
 
     Local Open Scope arrow_scope.
+    Local Open Scope category_scope.
 
     Inductive kappa : object -> object -> Type :=
-      | Var : forall {x y},   var x y -> kappa x y
-      | Abs : forall x {y z}, (var u x -> kappa y z) -> kappa (x ** y) z
-      | App : forall {x y z}, kappa (x ** y) z -> kappa u x -> kappa y z
-      | Comp: forall {x y z}, kappa y z -> kappa x y -> kappa x z
-      | Morph : forall {x y}, morphism x y -> kappa x y
-      | LetRec : forall x {y z}, 
-          (var u x -> kappa u x)
-        -> (var u x -> kappa y z) 
-        -> kappa y z.
+    | Var : forall {x y},   var x y -> kappa x y
+    | Abs : forall x {y z}, (var u x -> kappa y z) -> kappa (x ** y) z
+    | App : forall {x y z}, kappa (x ** y) z -> kappa u x -> kappa y z
+    | Comp: forall {x y z}, kappa y z -> kappa x y -> kappa x z
+    | Morph : forall {x y}, morphism x y -> kappa x y
+    | LetRec : forall x {y z}, 
+        (var u x -> kappa u x)
+      -> (var u x -> kappa y z) 
+      -> kappa y z.
+
+    Inductive NoLetRecKappa: forall i o, kappa i o -> Prop :=
+    | NoLetRecVar: forall x y v, NoLetRecKappa x y (Var v)
+    | NoLetRecAbs: forall x y z f,
+      (forall (k: var u x), NoLetRecKappa y z (f k)) -> NoLetRecKappa (x**y) z (Abs _ f)
+    | NoLetRecApp: forall x y z f e,
+      NoLetRecKappa (x ** y) z f -> NoLetRecKappa u x e -> NoLetRecKappa y z (App f e)
+    | NoLetRecComp: forall x y z f g,
+      NoLetRecKappa y z f -> NoLetRecKappa x y g -> NoLetRecKappa x z (Comp f g)
+    | NoLetRecMorph : forall x y m, NoLetRecKappa x y (Morph m).
+
+    Section prop.
+      Variable (P: forall x y, morphism x y -> Prop).
+
+      Inductive MorphPropKappa: forall i o, kappa i o -> Prop :=
+      | MorphPropVar: forall x y v, MorphPropKappa x y (Var v)
+      | MorphPropAbs: forall x y z f, (forall (k: var u x), MorphPropKappa y z (f k)) -> MorphPropKappa (x**y) z (Abs _ f)
+      | MorphPropApp: forall x y z f e,
+        MorphPropKappa (x ** y) z f -> MorphPropKappa u x e -> MorphPropKappa y z (App f e)
+      | MorphPropComp: forall x y z f g,
+        MorphPropKappa y z f -> MorphPropKappa x y g -> MorphPropKappa x z (Comp f g)
+      | MorphPropMorph : forall x y m, P x y m -> MorphPropKappa x y (Morph m).
+
+    End prop.
+
   End Vars.
 
   Definition Kappa i o := forall var, kappa var i o.
+
 End Arrow.
